continue

Superposition_Calculus/First_Order_Superposition.thy
@@ -17,8 +17,6 @@ hide_const
 
 section \<open>First-Order Layer\<close>
 
-type_synonym ('f, 'v, 'ty) typed_clause = "('f, 'v) atom clause \<times> ('v, 'ty) var_types"
-
 locale first_order_superposition_calculus =
   first_order_select select +
   first_order_ordering less\<^sub>t +
@@ -34,10 +32,21 @@ locale first_order_superposition_calculus =
       "\<And>clause\<^sub>G. wfP (tiebreakers clause\<^sub>G) \<and> 
                transp (tiebreakers clause\<^sub>G) \<and> 
                asymp (tiebreakers clause\<^sub>G)" and
-    ground_critical_pair_theorem: "\<And>(R :: 'f gterm rel). ground_critical_pair_theorem R"
+    ground_critical_pair_theorem: "\<And>(R :: 'f gterm rel). ground_critical_pair_theorem R" 
 begin
 
-inductive eq_resolution :: "('v, 'ty) var_types \<Rightarrow> ('f, 'v) atom clause \<Rightarrow> ('f, 'v) atom clause \<Rightarrow> bool" where
+abbreviation typed_tiebreakers ::  "'f gatom clause \<Rightarrow> ('f, 'v, 'ty) typed_clause \<Rightarrow> ('f, 'v, 'ty) typed_clause \<Rightarrow> bool" 
+  where "typed_tiebreakers clause\<^sub>G clause\<^sub>1 clause\<^sub>2 \<equiv> tiebreakers clause\<^sub>G (fst clause\<^sub>1) (fst clause\<^sub>2)"
+
+lemma wellfounded_typed_tiebreakers: 
+      "wfP (typed_tiebreakers clause\<^sub>G) \<and>  transp (typed_tiebreakers clause\<^sub>G) \<and>  asymp (typed_tiebreakers clause\<^sub>G)"
+  using wellfounded_tiebreakers
+  apply auto
+    apply (meson wfP_if_convertible_to_wfP)
+   apply (smt (verit, ccfv_threshold) transpD transpI)
+  by (meson asympD asympI)
+
+inductive eq_resolution :: "('f, 'v, 'ty) typed_clause \<Rightarrow> ('f, 'v, 'ty) typed_clause \<Rightarrow> bool" where
   eq_resolutionI: 
    "premise = add_mset literal premise' \<Longrightarrow>
     literal = term !\<approx> term' \<Longrightarrow>
@@ -46,9 +55,9 @@ inductive eq_resolution :: "('v, 'ty) var_types \<Rightarrow> ('f, 'v) atom clau
     select premise = {#} \<and> is_maximal\<^sub>l (literal \<cdot>l \<mu>) (premise \<cdot> \<mu>) \<or> 
       is_maximal\<^sub>l (literal \<cdot>l \<mu>) ((select premise) \<cdot> \<mu>) \<Longrightarrow>
     conclusion = premise' \<cdot> \<mu> \<Longrightarrow>
-    eq_resolution \<V> premise conclusion"
+    eq_resolution (premise, \<V>) (conclusion, \<V>)"
 
-inductive eq_factoring :: "('v, 'ty) var_types \<Rightarrow> ('f, 'v) atom clause \<Rightarrow> ('f, 'v) atom clause \<Rightarrow> bool" where
+inductive eq_factoring :: "('f, 'v, 'ty) typed_clause \<Rightarrow> ('f, 'v, 'ty) typed_clause \<Rightarrow> bool" where
   eq_factoringI: "
     premise = add_mset literal\<^sub>1 (add_mset literal\<^sub>2 premise') \<Longrightarrow>
     literal\<^sub>1 = term\<^sub>1 \<approx> term\<^sub>1' \<Longrightarrow>
@@ -60,11 +69,11 @@ inductive eq_factoring :: "('v, 'ty) var_types \<Rightarrow> ('f, 'v) atom claus
     welltyped_imgu typeof_fun \<V> term\<^sub>1 term\<^sub>2 \<mu> \<Longrightarrow>
     (welltyped\<^sub>c typeof_fun \<V> premise \<Longrightarrow> \<exists>\<tau>. has_type typeof_fun \<V> term\<^sub>1 \<tau> \<and> has_type typeof_fun \<V> term\<^sub>2 \<tau>) \<Longrightarrow>
     conclusion = add_mset (term\<^sub>1 \<approx> term\<^sub>2') (add_mset (term\<^sub>1' !\<approx> term\<^sub>2') premise') \<cdot> \<mu> \<Longrightarrow>
-    eq_factoring \<V> premise conclusion"
+    eq_factoring (premise, \<V>) (conclusion, \<V>)"
 
 (* TODO *)
 inductive superposition ::
-  "('v, 'ty) var_types \<Rightarrow> ('f, 'v) atom clause \<Rightarrow> ('v, 'ty) var_types \<Rightarrow> ('f, 'v) atom clause \<Rightarrow> ('f, 'v) atom clause \<Rightarrow> bool"
+  "('f, 'v, 'ty) typed_clause \<Rightarrow> ('f, 'v, 'ty) typed_clause \<Rightarrow> ('f, 'v, 'ty) typed_clause \<Rightarrow> bool"
 where
   superpositionI: 
    "term_subst.is_renaming \<rho>\<^sub>1 \<Longrightarrow>
@@ -92,30 +101,30 @@ where
     \<not> (term\<^sub>2 \<cdot>t \<rho>\<^sub>2 \<cdot>t \<mu> \<preceq>\<^sub>t term\<^sub>2' \<cdot>t \<rho>\<^sub>2 \<cdot>t \<mu>) \<Longrightarrow>
     conclusion = add_mset (\<P> (Upair (context\<^sub>1 \<cdot>t\<^sub>c \<rho>\<^sub>1)\<langle>term\<^sub>2' \<cdot>t \<rho>\<^sub>2\<rangle> (term\<^sub>1' \<cdot>t \<rho>\<^sub>1))) 
           (premise\<^sub>1' \<cdot> \<rho>\<^sub>1 + premise\<^sub>2' \<cdot> \<rho>\<^sub>2) \<cdot> \<mu> \<Longrightarrow>
-    superposition \<V>\<^sub>2 premise\<^sub>2 \<V>\<^sub>1 premise\<^sub>1 conclusion"
+    superposition (premise\<^sub>2, \<V>\<^sub>2) (premise\<^sub>1, \<V>\<^sub>1) (conclusion, \<V>\<^sub>1)"
 
 abbreviation eq_factoring_inferences where
   "eq_factoring_inferences \<equiv> 
-    { Infer [premise] conclusion | \<V> premise conclusion. eq_factoring \<V> premise conclusion }"
+    { Infer [premise] conclusion | premise conclusion. eq_factoring premise conclusion }"
 
 abbreviation eq_resolution_inferences where
   "eq_resolution_inferences \<equiv> 
-    { Infer [premise] conclusion | \<V> premise conclusion. eq_resolution \<V> premise conclusion }"
+    { Infer [premise] conclusion | premise conclusion. eq_resolution premise conclusion }"
 
 abbreviation superposition_inferences where
   "superposition_inferences \<equiv> { Infer [premise\<^sub>2, premise\<^sub>1] conclusion 
-    |  \<V>\<^sub>2 premise\<^sub>2 \<V>\<^sub>1 premise\<^sub>1 conclusion. superposition \<V>\<^sub>2 premise\<^sub>2 \<V>\<^sub>1 premise\<^sub>1 conclusion}"
+    |  premise\<^sub>2 premise\<^sub>1 conclusion. superposition premise\<^sub>2 premise\<^sub>1 conclusion}"
 
-definition inferences :: "('f, 'v) atom clause inference set" where
+definition inferences :: "('f, 'v, 'ty) typed_clause inference set" where
   "inferences \<equiv> superposition_inferences \<union> eq_resolution_inferences \<union> eq_factoring_inferences"
 
-abbreviation bottom\<^sub>F :: "('f, 'v) atom clause set" ("\<bottom>\<^sub>F") where
-  "bottom\<^sub>F \<equiv> {{#}}"
+abbreviation bottom\<^sub>F :: "('f, 'v, 'ty) typed_clause set" ("\<bottom>\<^sub>F") where
+  "bottom\<^sub>F \<equiv> {({#}, \<V>) | \<V>. True }"
 
 subsubsection \<open>Alternative Specification of the Superposition Rule\<close>
 
 inductive pos_superposition ::
-  "('v, 'ty) var_types \<Rightarrow> ('f, 'v) atom clause \<Rightarrow> ('v, 'ty) var_types \<Rightarrow> ('f, 'v) atom clause \<Rightarrow> ('f, 'v) atom clause \<Rightarrow> bool"
+  "('f, 'v, 'ty) typed_clause \<Rightarrow> ('f, 'v, 'ty) typed_clause \<Rightarrow> ('f, 'v, 'ty) typed_clause \<Rightarrow> bool"
 where
   pos_superpositionI: "
     term_subst.is_renaming \<rho>\<^sub>1 \<Longrightarrow>
@@ -137,11 +146,11 @@ where
     \<not> (s\<^sub>1\<langle>u\<^sub>1\<rangle> \<cdot>t \<rho>\<^sub>1 \<cdot>t \<mu> \<preceq>\<^sub>t s\<^sub>1' \<cdot>t \<rho>\<^sub>1 \<cdot>t \<mu>) \<Longrightarrow>
     \<not> (t\<^sub>2 \<cdot>t \<rho>\<^sub>2 \<cdot>t \<mu> \<preceq>\<^sub>t t\<^sub>2' \<cdot>t \<rho>\<^sub>2 \<cdot>t \<mu>) \<Longrightarrow>
     C = add_mset ((s\<^sub>1 \<cdot>t\<^sub>c \<rho>\<^sub>1)\<langle>t\<^sub>2' \<cdot>t \<rho>\<^sub>2\<rangle> \<approx> (s\<^sub>1' \<cdot>t \<rho>\<^sub>1)) (P\<^sub>1' \<cdot> \<rho>\<^sub>1 + P\<^sub>2' \<cdot> \<rho>\<^sub>2) \<cdot> \<mu> \<Longrightarrow>
-    pos_superposition \<V>\<^sub>2 P\<^sub>2 \<V>\<^sub>1 P\<^sub>1 C"
+    pos_superposition (P\<^sub>2, \<V>\<^sub>2) (P\<^sub>1, \<V>\<^sub>1) (C, \<V>\<^sub>1)"
 
 lemma superposition_if_pos_superposition:
-  assumes "pos_superposition \<V>\<^sub>2 P\<^sub>2 \<V>\<^sub>1 P\<^sub>1 C"
-  shows "superposition \<V>\<^sub>2 P\<^sub>2 \<V>\<^sub>1 P\<^sub>1 C"
+  assumes "pos_superposition P\<^sub>2 P\<^sub>1 C"
+  shows "superposition P\<^sub>2 P\<^sub>1 C"
   using assms
 proof (cases rule: pos_superposition.cases)
   case (pos_superpositionI \<rho>\<^sub>1 \<rho>\<^sub>2 L\<^sub>1 P\<^sub>1' L\<^sub>2 P\<^sub>2' s\<^sub>1 u\<^sub>1 s\<^sub>1' t\<^sub>2 t\<^sub>2' \<mu>)
@@ -151,7 +160,7 @@ proof (cases rule: pos_superposition.cases)
 qed
 
 inductive neg_superposition ::
-  "('v, 'ty) var_types \<Rightarrow> ('f, 'v) atom clause \<Rightarrow> ('v, 'ty) var_types \<Rightarrow> ('f, 'v) atom clause \<Rightarrow> ('f, 'v) atom clause \<Rightarrow> bool"
+  "('f, 'v, 'ty) typed_clause \<Rightarrow> ('f, 'v, 'ty) typed_clause \<Rightarrow> ('f, 'v, 'ty) typed_clause \<Rightarrow> bool"
 where
   neg_superpositionI: "
     term_subst.is_renaming \<rho>\<^sub>1 \<Longrightarrow>
@@ -173,13 +182,13 @@ where
     \<not> (s\<^sub>1\<langle>u\<^sub>1\<rangle> \<cdot>t \<rho>\<^sub>1 \<cdot>t \<mu> \<preceq>\<^sub>t s\<^sub>1' \<cdot>t \<rho>\<^sub>1 \<cdot>t \<mu>) \<Longrightarrow>
     \<not> (t\<^sub>2 \<cdot>t \<rho>\<^sub>2 \<cdot>t \<mu> \<preceq>\<^sub>t t\<^sub>2' \<cdot>t \<rho>\<^sub>2 \<cdot>t \<mu>) \<Longrightarrow>
     C = add_mset (Neg (Upair (s\<^sub>1 \<cdot>t\<^sub>c \<rho>\<^sub>1)\<langle>t\<^sub>2' \<cdot>t \<rho>\<^sub>2\<rangle>  (s\<^sub>1' \<cdot>t \<rho>\<^sub>1))) (P\<^sub>1' \<cdot> \<rho>\<^sub>1 + P\<^sub>2' \<cdot> \<rho>\<^sub>2) \<cdot> \<mu> \<Longrightarrow>
-    neg_superposition \<V>\<^sub>2 P\<^sub>2 \<V>\<^sub>1 P\<^sub>1 C"
+    neg_superposition (P\<^sub>2, \<V>\<^sub>2) (P\<^sub>1, \<V>\<^sub>1) (C, \<V>\<^sub>1)"
 
 lemma superposition_if_neg_superposition:
-  assumes "neg_superposition  \<V>\<^sub>2 P\<^sub>2 \<V>\<^sub>1 P\<^sub>1 C"
-  shows "superposition  \<V>\<^sub>2 P\<^sub>2 \<V>\<^sub>1 P\<^sub>1 C"
+  assumes "neg_superposition  P\<^sub>2 P\<^sub>1 C"
+  shows "superposition P\<^sub>2 P\<^sub>1 C"
   using assms
-proof (cases \<V>\<^sub>2 P\<^sub>2 \<V>\<^sub>1 P\<^sub>1 C rule: neg_superposition.cases)
+proof (cases P\<^sub>2 P\<^sub>1 C rule: neg_superposition.cases)
   case (neg_superpositionI \<rho>\<^sub>1 \<rho>\<^sub>2 L\<^sub>1 P\<^sub>1' L\<^sub>2 P\<^sub>2' s\<^sub>1 u\<^sub>1 s\<^sub>1' t\<^sub>2 t\<^sub>2' \<mu>)
   then show ?thesis
     using superpositionI
@@ -187,21 +196,21 @@ proof (cases \<V>\<^sub>2 P\<^sub>2 \<V>\<^sub>1 P\<^sub>1 C rule: neg_superposi
 qed
 
 lemma superposition_iff_pos_or_neg:
-  "superposition \<V>\<^sub>2 P\<^sub>2 \<V>\<^sub>1 P\<^sub>1 C \<longleftrightarrow> pos_superposition \<V>\<^sub>2 P\<^sub>2 \<V>\<^sub>1 P\<^sub>1 C \<or> neg_superposition \<V>\<^sub>2 P\<^sub>2 \<V>\<^sub>1 P\<^sub>1 C"
+  "superposition P\<^sub>2 P\<^sub>1 C \<longleftrightarrow> pos_superposition P\<^sub>2 P\<^sub>1 C \<or> neg_superposition P\<^sub>2  P\<^sub>1 C"
 proof (rule iffI)
-  assume "superposition \<V>\<^sub>2 P\<^sub>2 \<V>\<^sub>1 P\<^sub>1 C"
-  thus "pos_superposition \<V>\<^sub>2 P\<^sub>2 \<V>\<^sub>1 P\<^sub>1 C \<or> neg_superposition \<V>\<^sub>2 P\<^sub>2 \<V>\<^sub>1 P\<^sub>1 C"
-  proof (cases \<V>\<^sub>2 P\<^sub>2 \<V>\<^sub>1 P\<^sub>1 C rule: superposition.cases)
-    case (superpositionI \<rho>\<^sub>1 \<rho>\<^sub>2 literal\<^sub>1 premise\<^sub>1' literal\<^sub>2 premise\<^sub>2' \<P> context\<^sub>1 term\<^sub>1 term\<^sub>1' term\<^sub>2 term\<^sub>2' \<mu>)
+  assume "superposition P\<^sub>2 P\<^sub>1 C"
+  thus "pos_superposition  P\<^sub>2 P\<^sub>1 C \<or> neg_superposition P\<^sub>2 P\<^sub>1 C"
+  proof (cases P\<^sub>2 P\<^sub>1 C rule: superposition.cases)
+    case (superpositionI \<rho>\<^sub>1 \<rho>\<^sub>2 premise\<^sub>1 premise\<^sub>2 literal\<^sub>1 premise\<^sub>1' literal\<^sub>2 premise\<^sub>2' \<P> context\<^sub>1 term\<^sub>1 term\<^sub>1' term\<^sub>2 term\<^sub>2' \<mu> \<V>\<^sub>1 \<V>\<^sub>2 conclusion)
     then show ?thesis 
       using 
-        pos_superpositionI[of \<rho>\<^sub>1 \<rho>\<^sub>2 P\<^sub>1 P\<^sub>2 literal\<^sub>1 premise\<^sub>1' literal\<^sub>2 premise\<^sub>2' context\<^sub>1 term\<^sub>1 term\<^sub>1' term\<^sub>2 term\<^sub>2']
-        neg_superpositionI[of \<rho>\<^sub>1 \<rho>\<^sub>2 P\<^sub>1 P\<^sub>2 literal\<^sub>1 premise\<^sub>1' literal\<^sub>2 premise\<^sub>2' context\<^sub>1 term\<^sub>1 term\<^sub>1' term\<^sub>2 term\<^sub>2'] 
+        pos_superpositionI[of \<rho>\<^sub>1 \<rho>\<^sub>2 premise\<^sub>1 premise\<^sub>2 literal\<^sub>1 premise\<^sub>1' literal\<^sub>2 premise\<^sub>2' context\<^sub>1 term\<^sub>1 term\<^sub>1' term\<^sub>2 term\<^sub>2' \<mu> \<V>\<^sub>1 \<V>\<^sub>2]
+        neg_superpositionI[of \<rho>\<^sub>1 \<rho>\<^sub>2 premise\<^sub>1 premise\<^sub>2 literal\<^sub>1 premise\<^sub>1' literal\<^sub>2 premise\<^sub>2' context\<^sub>1 term\<^sub>1 term\<^sub>1' term\<^sub>2 term\<^sub>2' \<mu> \<V>\<^sub>1 \<V>\<^sub>2] 
       by blast
   qed
 next
-  assume "pos_superposition  \<V>\<^sub>2 P\<^sub>2 \<V>\<^sub>1 P\<^sub>1 C \<or> neg_superposition  \<V>\<^sub>2 P\<^sub>2 \<V>\<^sub>1 P\<^sub>1 C"
-  thus "superposition  \<V>\<^sub>2 P\<^sub>2 \<V>\<^sub>1 P\<^sub>1 C"
+  assume "pos_superposition P\<^sub>2 P\<^sub>1 C \<or> neg_superposition P\<^sub>2 P\<^sub>1 C"
+  thus "superposition P\<^sub>2 P\<^sub>1 C"
     using superposition_if_neg_superposition superposition_if_pos_superposition by metis
 qed
 
@@ -220,11 +229,11 @@ lemmas clause_renaming_exists =
 (* TODO: abbreviations without typeof_fun typeof_var *)
 lemma eq_resolution_preserves_typing:
   assumes
-    step: "eq_resolution \<V> D C" and
+    step: "eq_resolution (D, \<V>) (C, \<V>)" and
     wt_D: "welltyped\<^sub>c typeof_fun \<V> D"
   shows "welltyped\<^sub>c typeof_fun \<V> C"
   using step
-proof (cases \<V> D C rule: eq_resolution.cases)
+proof (cases "(D, \<V>)" "(C, \<V>)" rule: eq_resolution.cases)
   case (eq_resolutionI literal premise' "term" term' \<mu>)
   obtain \<tau> where \<tau>:
     "welltyped typeof_fun \<V> term \<tau>"
@@ -259,11 +268,11 @@ lemma welltyped_has_type:
 
 lemma eq_factoring_preserves_typing:
   assumes
-    step: "eq_factoring \<V> D C" and
+    step: "eq_factoring (D, \<V>) (C, \<V>)" and
     wt_D: "welltyped\<^sub>c typeof_fun \<V> D"
   shows "welltyped\<^sub>c typeof_fun \<V> C"
   using step
-proof (cases \<V> D C rule: eq_factoring.cases)
+proof (cases "(D, \<V>)" "(C, \<V>)" rule: eq_factoring.cases)
   case (eq_factoringI literal\<^sub>1 literal\<^sub>2 premise' term\<^sub>1 term\<^sub>1' term\<^sub>2 term\<^sub>2' \<mu>)
   
   obtain \<tau> where \<tau>:
